eNFA_Regex_equivalence_other.lean
@@ -16,753 +16,12 @@ variable {α : Type u} [Fintype α] [DecidableEq α]
 
 set_option linter.unusedSectionVars false
 
-
-namespace εNFA
-
-variable {α : Type u} {σ : Type v} (M : εNFA α σ) {S : Set σ} {s t u : σ} {a : α}
-
-
-
-end εNFA
-
 --------------------------
 -- THE OTHER DIRECTION: --
 --------------------------
 
 variable {α : Type u} [Fintype α] [DecidableEq α]
-
-
-def SingularStart  := 2
-def SingularAccept := 0
-
-def to_singular (A : εNFA α ℕ) : εNFA α ℕ := {
-    start  := { SingularStart }
-    accept := { SingularAccept }
-    step   := fun q c =>
-        let A' := A.to_1mod2
-        if q % 2 = 1 then
-            if q ∈ A'.accept && c = none then
-                A'.step q c ∪ { SingularAccept }
-            else
-                A'.step q c
-        else
-            if q = SingularStart && c = none then
-                A'.start
-            else
-                ∅
-    : εNFA α ℕ
-}
-
-def is_alone_in_set (set: Set ℕ) (n: ℕ):= set = { n }
-def is_singular (A : εNFA α ℕ) :=
-    (∃s: ℕ, is_alone_in_set A.start s) ∧ (∃a: ℕ, is_alone_in_set A.accept a)
-
-lemma to_singular_contains (A: εNFA α ℕ): (to_singular A).contains A.to_1mod2 := by
-    unfold εNFA.contains
-    intro q σ
-    simp [to_singular, εNFA.to_1mod2]
-    split_ifs
-    all_goals simp only [subset_insert, subset_refl, empty_subset]
-
-
-lemma accepts_iff_singular_accepts (A : εNFA α ℕ) (A' : εNFA α ℕ) (hA': A' = to_singular A) :
-    A.accepts = A'.accepts := by
-    rw [@Language.ext_iff]
-    intro x
-    constructor
-    case mp =>
-        intro h_A_accepts_x
-        rw[@εNFA.mem_accepts_iff_exists_path] at h_A_accepts_x ⊢
-
-        obtain ⟨ s, a, x', hs, ha, hx', hApath⟩ := h_A_accepts_x
-        use SingularStart, SingularAccept, ([none] ++ x' ++ [none])
-
-        refine ⟨ by subst hA'; rfl, by subst hA'; rfl,
-            by simp only [List.nil_append, List.reduceOption_cons_of_none, List.reduceOption_append, List.reduceOption_nil, List.append_nil, hx']
-            , ?_ ⟩
-
-        have hfirst: Nonempty (A'.Path SingularStart (2*s + 1) [none]) := by
-            subst hA'
-            simp [to_singular, εNFA.to_1mod2, hs, SingularStart]
-
-        have hlast: Nonempty (A'.Path (2*a + 1) SingularAccept [none]) := by
-            subst hA'
-            simp [to_singular, εNFA.to_1mod2, ha, SingularAccept]
-
-        have hmiddle: Nonempty (A'.Path (2*s + 1) (2*a + 1) x') := by
-            subst hA'
-            have h_A_0mod2_path := (A.path_iff_1mod2_path A.to_1mod2 s a (2*s + 1) (2*a + 1) x' rfl rfl rfl).mp hApath
-            have hcontains := to_singular_contains A
-            apply εNFA.path_if_contains at hcontains
-            exact hcontains (2*s + 1) (2*a + 1) x' h_A_0mod2_path
-
-        apply A'.isPath_append.mpr; use (2*a + 1)
-        refine ⟨ ?_, hlast ⟩
-
-        apply A'.isPath_append.mpr; use (2*s + 1)
-
-    case mpr =>
-        intro h_A'_accepts_x
-        rw [A.accepts_iff_1mod2_accepts A.to_1mod2 rfl]
-
-        rw[@εNFA.mem_accepts_iff_exists_path] at h_A'_accepts_x ⊢
-        obtain ⟨ s', a', x', h_s'_start, h_a'_accept, h_x', hA'path ⟩ := h_A'_accepts_x
-
-        have h_s'_2: s' = SingularStart := by
-            subst hA'
-            simp [to_singular] at h_s'_start
-            exact h_s'_start
-
-        have h_a'_4: a' = SingularAccept := by
-            subst hA'
-            simp [to_singular] at h_a'_accept
-            exact h_a'_accept
-
-        subst h_s'_2
-        subst h_a'_4
-        clear h_s'_start h_a'_accept
-
-        obtain ⟨ hA'path ⟩ := hA'path
-        cases hA'path
-        case cons s σ y' h_step h_path_s_accept =>
-            simp [hA', to_singular, SingularStart, SingularAccept] at h_step
-            obtain ⟨ ⟨ _, h_σ_none ⟩ , h_s_start ⟩ := h_step
-
-            have first_transition_is_to_odd_state: s % 2 = 1:=
-                A.to_1mod2.if_1mod2_qs_is_1mod2 ⟨A, rfl⟩ s h_s_start
-
-            have h_temp: ∀ (q q': ℕ) (σ : Option α), (q % 2 = 1) → (q' % 2 = 1) → (q' ∈ A'.step q σ )
-            → (q' ∈ A.to_1mod2.step q σ ) := by
-                intro q q' σ hq_odd hq'_odd hstep
-                subst hA'
-                simp [to_singular, hq_odd] at hstep ⊢
-                by_cases hacc : q ∈ (A.to_1mod2).accept ∧ σ = none
-                · simp [hacc] at hstep ⊢
-                  rcases hstep with h | h
-                  · exfalso
-                    simp[SingularAccept] at h
-                    omega
-                  · exact h
-                · simp [hacc] at hstep ⊢
-                  exact hstep
-
-               --transition between odds in A' -> same transition in A1
-
-            --next step: path between odds in A' is odd
-            --next step: odd path in A' -> odd path in A1
-
-            have path_to_singular_accept (q : ℕ) (y : List (Option α))
-                (h_q_1mod2: q % 2 = 1) (h_path : Nonempty (A'.Path q SingularAccept y)) :
-                ∃ qf mid, qf ∈ (A.to_1mod2).accept ∧ (Nonempty (A.to_1mod2.Path q qf mid)) ∧ y = mid ++ [none] := by
-                induction y generalizing q
-                case nil =>
-                    simp only [εNFA.isPath_nil] at h_path
-                    simp [SingularAccept] at h_path
-                    omega
-                case cons c tail h_induction =>
-                    obtain ⟨ h_path ⟩ := h_path
-                    cases h_path
-                    case cons t h_step h_path =>
-                        by_cases tail = []
-                        case pos h_tail_empty =>
-                            clear h_induction
-                            subst h_tail_empty
-                            replace h_path : Nonempty (A'.Path t SingularAccept []) := by use h_path
-                            simp only [εNFA.isPath_nil] at h_path
-                            subst h_path
-
-                            have h_c_none : c = none := by
-                                simp [hA', to_singular, h_q_1mod2] at h_step
-                                split_ifs at h_step
-                                case pos h_none => exact h_none.right
-                                case neg =>
-                                    have : SingularAccept % 2 = 1 :=
-                                        (A.to_1mod2.if_1mod2_step_is_1mod2 ⟨A,rfl⟩ q SingularAccept c h_step).right
-                                    simp [SingularAccept] at this -- contradiction
-                            subst h_c_none
-
-                            use q, []
-                            simp only [εNFA.isPath_nil, List.nil_append, and_self, and_true]
-
-                            simp [hA', to_singular, h_q_1mod2] at h_step
-                            split_ifs at h_step
-                            case pos h_q_accept => exact h_q_accept
-                            case neg =>
-                                have : SingularAccept % 2 = 1 :=
-                                        (A.to_1mod2.if_1mod2_step_is_1mod2 ⟨A,rfl⟩ q SingularAccept none h_step).right
-                                simp [SingularAccept] at this -- contradiction
-
-                        case neg h_tail_nonempty =>
-                            have h_t_1mod2 : t % 2 = 1 := by
-                                cases h_path
-                                case nil => contradiction
-                                case cons t' c' tail' h_step' h_path' =>
-                                    have h_t_not_SAS : t ≠ SingularAccept := by
-                                        by_contra!
-                                        subst this
-
-                                        have h_step'_empty : A'.step SingularAccept c' = ∅ := by
-                                            simp [hA', to_singular, SingularAccept, SingularStart]
-
-                                        simp [h_step'_empty] at h_step' --contradiction
-
-                                    simp [hA', to_singular, h_q_1mod2] at h_step
-                                    split_ifs at h_step
-                                    case pos h_accept =>
-                                        simp [h_t_not_SAS] at h_step
-                                        exact (A.to_1mod2.if_1mod2_step_is_1mod2 ⟨A, rfl⟩ q t c h_step).right
-                                    case neg => exact (A.to_1mod2.if_1mod2_step_is_1mod2 ⟨A, rfl⟩ q t c h_step).right
-
-                            replace h_path: Nonempty (A'.Path t SingularAccept tail) := by use h_path
-                            obtain ⟨ qf, mid', h_induction ⟩ := h_induction t h_t_1mod2 h_path
-                            use qf, c :: mid'
-                            simp [h_induction]
-                            replace h_induction := h_induction.right.left
-                            simp [hA', to_singular, h_q_1mod2] at h_step
-                            split_ifs at h_step
-                            case pos =>
-                                have : t ≠ SingularAccept := by simp [SingularAccept]; omega
-                                simp [this] at h_step
-                                apply A.to_1mod2.isPath_singleton.mpr at h_step
-                                exact A.to_1mod2.isPath_append.mpr ⟨ t, h_step, h_induction⟩
-                            case neg =>
-                                apply A.to_1mod2.isPath_singleton.mpr at h_step
-                                exact A.to_1mod2.isPath_append.mpr ⟨ t, h_step, h_induction⟩
-
-            replace h_path_s_accept: Nonempty (A'.Path s SingularAccept y') := by use h_path_s_accept
-            obtain ⟨qf, mid, h_qf_accept, h_mid_path, h_y'_eq⟩ :=
-              path_to_singular_accept (q := s) (y := y') first_transition_is_to_odd_state h_path_s_accept
-
-            have h_mid : mid.reduceOption = x := by
-                simp only [h_y'_eq, List.reduceOption_cons_of_none, List.reduceOption_append,
-                  List.reduceOption_nil, List.append_nil] at h_x'
-                exact h_x'
-
-            use s, qf, mid
-
-
-def εNFA.max_reachable_node (A : εNFA α ℕ) (n : ℕ) :=
-    (∃s₁: ℕ, ∃x: List (Option α), s₁ ∈ A.start ∧ Nonempty (A.Path s₁ n x))
-    ∧
-    ∀n': ℕ, (n' > n) → ¬(∃s₁: ℕ, ∃x: List (Option α), s₁ ∈ A.start ∧ Nonempty (A.Path s₁ n' x))
-
-def εNFA.is_finite_automata (A : εNFA α ℕ) :=
-    (A.start = ∅) ∨ (∃n: ℕ, A.max_reachable_node n)
-
-lemma if_1mod2_max_reachable_is_1mod2 (A : εNFA α ℕ) (n: ℕ) (hA: A.is_1mod2) (h_n: A.max_reachable_node n) :
-    n % 2 = 1 := by
-    unfold εNFA.max_reachable_node at h_n
-    obtain ⟨ ⟨ s, x, ⟨ h_s_start, h_path ⟩ ⟩, _ ⟩ := h_n
-    apply A.if_1mod2_qs_is_1mod2 hA at h_s_start
-    apply A.if_1mod2_path_is_same_mod2 hA s n x at h_path
-    omega
-
-lemma finite_iff_1mod2_is_finite (A : εNFA α ℕ) (A' : εNFA α ℕ) (hA': A' = A.to_1mod2) :
-    A.is_finite_automata ↔ A'.is_finite_automata := by
-    constructor
-    case mp =>
-        intro h_A_is_finite
-        unfold εNFA.is_finite_automata at h_A_is_finite ⊢
-        cases h_A_is_finite
-        case inl h_A_start_empty =>
-            left
-            simp [hA', εNFA.to_1mod2, h_A_start_empty]
-        case inr h_max_reachable =>
-            right
-            obtain ⟨ n, h_max_reachable ⟩ := h_max_reachable
-            use 2*n + 1
-            unfold εNFA.max_reachable_node at h_max_reachable ⊢
-            obtain ⟨ ⟨ s, x, ⟨ h_s_start, h_path ⟩ ⟩, h ⟩ := h_max_reachable
-            have h_A_path_iff_A'_path := (A.path_iff_1mod2_path A' s n (2*s + 1) (2*n + 1) x hA' rfl rfl).mp h_path
-            constructor
-            case left =>
-                use 2*s + 1, x
-                exact ⟨ by simp [hA', εNFA.to_1mod2, h_s_start], h_A_path_iff_A'_path ⟩
-            case right =>
-                intro k' h_k'
-                by_cases k' % 2 = 0
-                case pos h_k'_0mod2 =>
-                    simp
-                    intro s' h_s' x
-                    by_contra! h_A'_path
-
-                    replace h_s' := A'.if_1mod2_qs_is_1mod2 ⟨A, hA'⟩ s' h_s'
-                    have := A'.if_1mod2_path_is_same_mod2 ⟨A, hA'⟩ s' k' x h_A'_path
-                    omega
-
-                case neg =>
-                    let k := (k' - 1)/2
-
-                    have h_k_greater: k > n := by omega
-                    have h_path_A := h k h_k_greater
-                    simp at h_path_A ⊢
-                    intro s' h_s' x
-
-                    simp [hA', εNFA.to_1mod2] at h_s'
-                    obtain ⟨ s, h_s_start, h_s ⟩ := h_s'
-                    replace h_path_A := h_path_A s h_s_start x
-                    replace h_k': k' = 2*k + 1 := by omega
-                    by_contra! h_path_A'
-                    have := (A.path_iff_1mod2_path A' s k s' k' x hA' (symm h_s) h_k').mpr h_path_A'
-                    absurd h_path_A
-                    simp only [not_isEmpty_of_nonempty, not_false_eq_true]
-
-    case mpr =>
-        intro h_A'_is_finite
-        unfold εNFA.is_finite_automata at h_A'_is_finite ⊢
-        cases h_A'_is_finite
-        case inl h_A'_start_empty =>
-            left
-            by_contra! h_A_start_nonempty
-            obtain ⟨ q, h_q ⟩ := nonempty_def.mp h_A_start_nonempty
-            clear h_A_start_nonempty
-            absurd h_A'_start_empty
-            push_neg
-            simp [nonempty_def]
-            use 2*q + 1
-            simp [hA', εNFA.to_1mod2, h_q]
-
-        case inr h_max_reachable =>
-            right
-            obtain ⟨n', h_max_reachable⟩ := h_max_reachable
-            have h_n'_1mod2 : n' % 2 = 1 := if_1mod2_max_reachable_is_1mod2 A' n' ⟨A, hA'⟩ h_max_reachable
-
-            let n := (n' - 1) / 2
-            use n
-            unfold εNFA.max_reachable_node at h_max_reachable ⊢
-            constructor
-            case left =>
-                obtain ⟨ ⟨ s', x, ⟨ h_s'_start, h_A'_path ⟩ ⟩, _ ⟩ := h_max_reachable
-                simp [hA', εNFA.to_1mod2] at h_s'_start
-                obtain ⟨s, h_s ⟩ := h_s'_start
-                use s, x
-
-                refine ⟨ h_s.left, ?_ ⟩
-                have := A.path_iff_1mod2_path A' s n s' n' x hA' (symm h_s.right) (by omega)
-                exact this.mpr h_A'_path
-
-            case right =>
-                obtain ⟨ ⟨_ ⟩, h ⟩ := h_max_reachable
-                intro k h_k
-                let k' := k*2 + 1
-                simp
-                intro s h_s x
-                by_contra! h_path_A
-                have := h k' (by omega)
-                absurd this
-
-                let s' := s*2 + 1
-                have h_s'_start: s' ∈ A'.start := by
-                    simp [hA', εNFA.to_1mod2, s']
-                    use s
-                    exact ⟨h_s, by omega⟩
-
-                use s', x
-                refine ⟨ h_s'_start, ?_ ⟩
-                have := A.path_iff_1mod2_path A' s k s' k' x hA' (by omega) (by omega)
-                exact this.mp h_path_A
-
-lemma if_singular_1mod2_path (A A' : εNFA α ℕ) (qs qf : ℕ) (hA': A' = to_singular A)
-    (h_qs: qs % 2 = 1) (h_qf: qf % 2 = 1) (x: List (Option α)):
-    Nonempty (A'.Path qs qf x) ↔ Nonempty (A.to_1mod2.Path qs qf x) := by
-    constructor
-    case mp =>
-        intro h_A'_path
-        obtain ⟨ h_A'_path ⟩ := h_A'_path
-        induction h_A'_path
-        case nil => simp only [εNFA.isPath_nil]
-        case cons t qs qf c tail h_step h_path h_induction =>
-            have h_t : t % 2 = 1 := by
-                clear h_induction
-                by_contra!
-                simp [hA', to_singular, h_qs] at h_step
-                split_ifs at h_step
-                case pos h_c_none =>
-                    simp at h_step
-                    cases h_step
-                    case inl h_t_singular =>
-                        replace h_c_none := h_c_none.right
-                        subst h_c_none
-
-                        have h_t_step :∀ (c: Option α), A'.step t c = ∅ := by
-                            simp [h_t_singular, hA', to_singular, SingularAccept, SingularStart]
-
-                        cases h_path
-                        case nil => contradiction
-                        case cons t' c tail' h_step' _ =>
-                            replace h_t_step := h_t_step c
-                            simp [h_t_step] at h_step' -- contradiction
-
-                    case inr h_step =>
-                        have := A.to_1mod2.if_1mod2_step_is_1mod2 ⟨A, rfl⟩ qs t c h_step
-                        omega
-
-                case neg =>
-                    have := A.to_1mod2.if_1mod2_step_is_1mod2 ⟨A, rfl⟩ qs t c h_step
-                    omega
-
-            replace h_step : t ∈ A.to_1mod2.step qs c := by
-                simp [hA', to_singular, h_qs, SingularAccept, SingularStart] at h_step
-                split_ifs at h_step
-                case pos =>
-                    simp at h_step
-                    cases h_step
-                    case inl => omega
-                    case inr h_step=>  exact h_step
-                case neg => exact h_step
-
-            apply A.to_1mod2.isPath_singleton.mpr at h_step
-            have := h_induction h_t h_qf
-            exact A.to_1mod2.isPath_append.mpr ⟨ t, h_step, this ⟩
-
-    case mpr =>
-        intro h_A1mod2_path
-
-        have h_A'_contains_A_1mod2 : A'.contains A.to_1mod2 := by
-            subst hA'
-            exact to_singular_contains A
-
-        exact A'.path_if_contains A.to_1mod2 h_A'_contains_A_1mod2 qs qf x h_A1mod2_path
-
-lemma singular_path_from_odd_ends_odd
-    (A A' : εNFA α ℕ) (q qf : ℕ) (y : List (Option α))
-    (hA' : A' = to_singular A)
-    (h_q_odd : q % 2 = 1)
-    (h_qf_gt : qf > SingularStart)
-    (h_path : Nonempty (A'.Path q qf y)) :
-    qf % 2 = 1 := by
-  obtain ⟨ h_path ⟩ := h_path
-  induction h_path
-  · omega
-  · rename_i t q qf c tail h_step h_rest ih
-    by_cases h_tail_empty : tail = []
-    · subst h_tail_empty
-      replace h_rest : Nonempty (A'.Path t qf []) := by use h_rest
-      apply A'.isPath_nil.mp at h_rest
-
-      subst h_rest
-      have h_t_ne_zero : t ≠ SingularAccept := by
-        simp [SingularAccept]
-        omega
-
-      simp [hA', to_singular, h_q_odd, SingularAccept, SingularStart] at h_step h_t_ne_zero
-      split_ifs at h_step
-      · simp [h_t_ne_zero] at h_step
-        exact (A.to_1mod2.if_1mod2_step_is_1mod2 ⟨A, rfl⟩ q t c h_step).right
-      · exact (A.to_1mod2.if_1mod2_step_is_1mod2 ⟨A, rfl⟩ q t c h_step).right
-    · have h_t_odd : t % 2 = 1 := by
-        simp [hA', to_singular, h_q_odd] at h_step
-        split_ifs at h_step
-        · rcases h_step with h_zero | h_step1
-          · subst h_zero
-            cases h_rest with
-            | nil => contradiction
-            | cons =>
-                rename_i u d tail' hstep_bad hpath_bad
-                simp [hA', to_singular, SingularAccept, SingularStart] at hstep_bad
-          · exact (A.to_1mod2.if_1mod2_step_is_1mod2 ⟨A, rfl⟩ q t c h_step1).right
-        · exact (A.to_1mod2.if_1mod2_step_is_1mod2 ⟨A, rfl⟩ q t c h_step).right
-      exact ih h_t_odd h_qf_gt
-
-lemma finite_iff_to_singular_finite (A A' : εNFA α ℕ) (hA': A' = to_singular A):
-    A.is_finite_automata ↔ A'.is_finite_automata := by
-    rw [finite_iff_1mod2_is_finite A A.to_1mod2 rfl]
-
-    unfold εNFA.is_finite_automata
-    constructor
-    case mp =>
-        rintro (h_start_empty | h_max_reachable)
-        case inl =>
-            right
-
-            use SingularStart
-            unfold εNFA.max_reachable_node
-            constructor
-            case h.left =>
-                use SingularStart, []
-                simp [hA', to_singular]
-            case h.right =>
-                intro n' h_n'
-                by_contra!
-                obtain ⟨ s₁, x, h ⟩ := this
-                have : s₁ = SingularStart := by
-                    replace h := h.left
-                    simp [hA', to_singular] at h
-                    exact h
-                subst this
-                replace h := h.right
-                obtain ⟨ h ⟩ := h
-                cases h
-                case nil =>
-                    contradiction
-                case cons t c x' h_step h_path =>
-                    simp [hA', to_singular, h_start_empty, SingularStart] at h_step
-
-        case inr =>
-            right
-            obtain ⟨ n, h_n ⟩ := h_max_reachable
-
-            unfold εNFA.max_reachable_node at h_n ⊢
-
-            obtain ⟨ ⟨ q, x, h_q_start, h_path_q_n_x ⟩, h_n_max ⟩ := h_n
-
-            have h_A'_contains_A_1mod2 := to_singular_contains A
-            rw[← hA'] at h_A'_contains_A_1mod2
-
-            by_cases n > SingularStart
-            case pos =>
-                use n
-                constructor
-                case left =>
-                    use SingularStart, [none] ++ x
-                    refine ⟨ by simp [hA', to_singular], ?_ ⟩
-                    apply A'.path_if_contains A.to_1mod2 h_A'_contains_A_1mod2 at h_path_q_n_x
-
-                    have h_step: q ∈ A'.step SingularStart none := by
-                        simp [hA', to_singular, SingularStart, h_q_start]
-
-                    apply A'.isPath_singleton.mpr at h_step
-                    exact A'.isPath_append.mpr ⟨ q, h_step, h_path_q_n_x ⟩
-
-                case right =>
-                    intro n' h_n'
-
-                    simp at h_n_max ⊢
-                    intro s' h_s' x
-
-                    simp [hA', to_singular] at h_s'
-                    subst h_s'
-
-                    by_contra!
-                    obtain ⟨ this ⟩ := this
-                    cases this
-                    case nil =>
-                        omega
-                    case cons t' c tail h_step h_path =>
-                        have h_t_start: t' ∈ A.to_1mod2.start := by
-                            simp [hA', to_singular, SingularStart] at h_step
-                            exact h_step.right
-
-                        absurd h_n_max
-                        simp
-                        use n'
-                        have : n' > n := by omega
-                        simp [this]
-                        clear this
-
-                        use t'
-
-                        refine ⟨ h_t_start, ?_ ⟩
-                        use tail
-                        by_cases h_tail_empty: tail = []
-                        case pos =>
-                            subst h_tail_empty
-                            replace h_path : Nonempty (A'.Path t' n' []) := by use h_path
-                            simp [A'.isPath_nil] at h_path ⊢
-                            exact h_path
-                        case neg =>
-                            have h_t' : t' % 2 = 1 := A.to_1mod2.if_1mod2_qs_is_1mod2 ⟨A, rfl⟩ t' h_t_start
-                            have h_n' : n' % 2 = 1 := by
-                                clear h_step h_n_max h_t_start
-                                induction h_path
-                                case nil => omega
-                                case cons t t' n' c tail' h_step h_path h_induction =>
-                                    by_cases h_tail'_empty: tail' = []
-                                    case pos =>
-                                        subst h_tail'_empty
-                                        replace h_path : Nonempty (A'.Path t n' []) := by use h_path
-                                        simp at h_path
-                                        subst h_path
-                                        have : t ≠ SingularAccept := by
-                                            have : SingularStart > SingularAccept := by
-                                                simp [SingularStart, SingularAccept]
-                                            omega
-                                        simp [hA', to_singular, h_t'] at h_step
-                                        split_ifs at h_step
-                                        case pos =>
-                                            simp [this] at h_step
-                                            exact (A.to_1mod2.if_1mod2_step_is_1mod2 ⟨A, rfl⟩ t' t c h_step).right
-                                        case neg =>
-                                            exact (A.to_1mod2.if_1mod2_step_is_1mod2 ⟨A, rfl⟩ t' t c h_step).right
-
-                                    case neg =>
-                                        apply h_induction h_n' h_tail'_empty
-                                        simp [hA', to_singular, h_t'] at h_step
-                                        split_ifs at h_step
-                                        case pos h_accept =>
-                                            replace h_accept := h_accept.left
-                                            simp at h_step
-                                            cases h_step
-                                            case inl h_t_accept =>
-                                                subst h_t_accept
-                                                cases h_path
-                                                case nil => contradiction
-                                                case cons u c _ h_step _ =>
-                                                    simp [hA', to_singular, SingularAccept, SingularStart] at h_step -- contradiction
-
-                                            case inr h_step =>
-                                                exact (A.to_1mod2.if_1mod2_step_is_1mod2 ⟨A, rfl⟩ t' t c h_step).right
-                                        case neg =>
-                                            exact (A.to_1mod2.if_1mod2_step_is_1mod2 ⟨A, rfl⟩ t' t c h_step).right
-
-                            replace h_path : Nonempty (A'.Path t' n' tail) := by use h_path
-                            exact (if_singular_1mod2_path A A' t' n' hA' h_t' h_n' tail).mp h_path
-            case neg =>
-                use SingularStart
-                constructor
-                case left =>
-                    use SingularStart, []
-                    simp [hA', to_singular]
-                case right  h_n_less =>
-                    simp at h_n_less
-                    intro n' h_n'
-
-                    have h_not_reach : ¬ ∃ s₁ x, s₁ ∈ A.to_1mod2.start ∧ Nonempty (A.to_1mod2.Path s₁ n' x) := by
-                        exact h_n_max n' (by omega)
-
-                    rintro ⟨ q, x, h_q_start, h_A'_path ⟩
-                    have h_q : q = SingularStart := by
-                        simp [hA', to_singular] at h_q_start
-                        exact h_q_start
-                    subst h_q
-                    obtain ⟨ h_A'_path ⟩ := h_A'_path
-                    cases h_A'_path with
-                    | nil =>
-                        omega
-                    | cons =>
-                        rename_i t' σ tail hstep hpath
-                        replace hpath : Nonempty (A'.Path t' n' tail) := by use hpath
-                        have h_t_start : t' ∈ A.to_1mod2.start := by
-                            simp [hA', to_singular, SingularStart] at hstep
-                            exact hstep.2
-                        have h_t_odd : t' % 2 = 1 :=
-                            A.to_1mod2.if_1mod2_qs_is_1mod2 ⟨A, rfl⟩ t' h_t_start
-                        have h_n'_odd : n' % 2 = 1 := by
-                             exact singular_path_from_odd_ends_odd A A' t' n' tail hA' h_t_odd h_n' hpath
-                        have h_path_1mod2 : Nonempty (A.to_1mod2.Path t' n' tail) :=
-                            (if_singular_1mod2_path A A' t' n' hA' h_t_odd h_n'_odd tail).mp hpath
-
-                        exact h_not_reach ⟨ t', tail, h_t_start, h_path_1mod2 ⟩
-
-    case mpr =>
-        rintro (h_start_empty | h_max_reachable)
-        case inl =>
-            exfalso
-            rw [hA'] at h_start_empty
-            simp [to_singular] at h_start_empty
-        case inr =>
-            have h_A'_contains_A_1mod2 := to_singular_contains A
-            rw[← hA'] at h_A'_contains_A_1mod2
-
-            by_cases h_start_empty : A.to_1mod2.start = ∅
-            case pos =>
-                exact Or.inl h_start_empty
-            case neg =>
-                right
-                obtain ⟨n, h_n⟩ := h_max_reachable
-                unfold εNFA.max_reachable_node at h_n ⊢
-                obtain ⟨h_n_reachable, h_n_max⟩ := h_n
-                obtain ⟨s, x, h_s_start, h_path⟩ := h_n_reachable
-                have h_bound :
-                ∀ k s x, s ∈ A.to_1mod2.start → Nonempty (A.to_1mod2.Path s k x) → k ≤ n := by
-                    intro k s x h_s_start h_path_1mod2
-                    by_contra h_not_le
-                    have hk_gt : k > n := by omega
-                    have h_step_from_singular : s ∈ A'.step SingularStart none := by
-                        simp [hA', to_singular, SingularStart, h_s_start]
-                    have h_singleton : Nonempty (A'.Path SingularStart s [none]) := by
-                        apply A'.isPath_singleton.mpr
-                        exact h_step_from_singular
-                    have h_path_in_A' : Nonempty (A'.Path s k x) := by
-                        exact A'.path_if_contains A.to_1mod2 h_A'_contains_A_1mod2 s k x h_path_1mod2
-                    have h_reach_k_in_A' : Nonempty (A'.Path SingularStart k ([none] ++ x)) := by
-                        exact A'.isPath_append.mpr ⟨s, h_singleton, h_path_in_A'⟩
-                    have h_not_reach := h_n_max k hk_gt
-                    apply h_not_reach
-                    use SingularStart, [none] ++ x
-                    constructor
-                    · simp [hA', to_singular]
-                    · exact h_reach_k_in_A'
-                have h_nonempty : ∃ s, s ∈ A.to_1mod2.start := by
-                    by_contra h_no_s
-                    apply h_start_empty
-                    rw [Set.eq_empty_iff_forall_notMem]
-                    intro s hs
-                    exact h_no_s ⟨s, hs⟩
-                obtain ⟨s, h_s_start⟩ := h_nonempty
-
-                let R : ℕ → Prop :=
-                    fun k => ∃ s₁ x,
-                        s₁ ∈ A.to_1mod2.start ∧
-                        Nonempty (A.to_1mod2.Path s₁ k x)
-
-                have hR_nonempty_bounded : ∃ k ≤ n, R k := by
-                    use s
-                    constructor
-                    · exact h_bound s s [] h_s_start ((A.to_1mod2.isPath_nil).mpr rfl)
-                    · unfold R
-                      use s, []
-                      exact ⟨h_s_start, (A.to_1mod2.isPath_nil).mpr rfl⟩
-
-                let m := Nat.findGreatest R n
-
-                use m
-
-                constructor
-                · unfold m
-                  obtain ⟨k, hk_le_n, hk_R⟩ := hR_nonempty_bounded
-                  exact Nat.findGreatest_spec hk_le_n hk_R
-
-                · intro k hk
-                  by_contra h_reach_k
-
-                  have hk_le_n : k ≤ n := by
-                    obtain ⟨s₁, x, h_s₁_start, h_path⟩ := h_reach_k
-                    exact h_bound k s₁ x h_s₁_start h_path
-
-                  have h_not_reach_k : ¬ R k := by
-                    unfold m at hk
-                    exact Nat.findGreatest_is_greatest hk hk_le_n
-
-                  exact h_not_reach_k h_reach_k
-
-def to_trim (A : εNFA α ℕ) (i j k : ℕ) : εNFA α ℕ := {
-    start  := { i }
-    accept := { j }
-    step   := fun q c =>
-        if j > k then
-            { q' | q' ∈ (A.step q c) ∧ ((q' ≤ k) ∨ (q' = j)) }
-        else
-            { q' | q' ∈ (A.step q c) ∧ ((q' ≤ k)) }
-    : εNFA α ℕ
-}
-
-def is_trim (A' : εNFA α ℕ) (i' j' k' : ℕ) :=
-    ∃ (A : εNFA α ℕ), A' = to_trim A i' j' k'
-
-def to_trim_contains (A A' : εNFA α ℕ) (i' j' k' : ℕ)
-    (h_trim : A' = to_trim A i' j' k') : A.contains A' := by
-    unfold εNFA.contains
-    intro q σ
-    subst h_trim
-    unfold to_trim
-    simp
-    split_ifs
-    case pos => simp
-    case neg => simp
-
-def path_if_to_trim_path (A A' : εNFA α ℕ) (qs qf i' j' k' : ℕ) (y : List (Option α))
-    (h_trim : A' = to_trim A i' j' k'):
-    Nonempty (A'.Path qs qf y) → Nonempty (A.Path qs qf y) := by
-    have h_contains := to_trim_contains A A' i' j' k' h_trim
-    exact εNFA.path_if_contains A A' h_contains qs qf y
-
-
-lemma singular_finite_accepts_iff_trim_accepts (A A': εNFA α ℕ) (s a n: ℕ)
-(hAsingular: is_singular A) (hAfinite: A.is_finite_automata)
-(hn_max: A.max_reachable_node n) (hs_start: is_alone_in_set A.start s) (ha_accept: is_alone_in_set A.accept a)
-(hA'istrim: A' = to_trim A s a n):
-    A.accepts = A'.accepts := by sorry -- TODO: EYAL
+open εNFA
 
 def character_list_to_regex : List α → RegularExpression α
     | .nil => 0
@@ -847,184 +106,14 @@ termination_by k
 decreasing_by
     all_goals omega
 
-lemma regex_for_path_contains_ij (A : εNFA α ℕ) (i j k k' : ℕ) (h_k' : k' ≤ k) :
-    (to_trim A i j k).contains (to_trim A i j k') := by
-    simp [εNFA.contains]
-    intro q σ
-    rw [@subset_def]
-    intro t h_step
-    simp [to_trim] at h_step ⊢
-    split_ifs
-    case pos h_k_j =>
-        have h_k'_j: k' < j := by omega
-        simp [h_k'_j] at h_step ⊢
-        cases h_step
-        case inl h_t_k' =>
-            left
-            simp [h_t_k']
-            omega
-        case inr h_t_j =>
-            right
-            exact h_t_j
-    case neg h_k_j =>
-        simp at h_k_j
-        split_ifs at h_step
-        case pos h_k'_j =>
-            simp at h_step
-            cases h_step
-            case inl h_step =>
-                simp [h_step.left]
-                omega
-            case inr h_step =>
-                simp [h_step.left]
-                omega
-        case neg h_k'_j =>
-            simp at h_k'_j h_step ⊢
-            simp [h_step.left]
-            omega
-
-lemma regex_for_path_contains_ik (A : εNFA α ℕ) (i j k k' : ℕ) (h_k' : k' ≤ k) :
-    (to_trim A i j k).contains (to_trim A i k k') := by
-    simp [εNFA.contains]
-    intro q σ
-    rw [@subset_def]
-    intro t h_step
-    simp [to_trim] at h_step ⊢
-    split_ifs
-    case pos h_k_j =>
-        have h_k'_j: k' < j := by omega
-        simp
-        split_ifs at h_step
-        case pos h_k'_less =>
-            left
-            simp_all
-            cases h_step
-            case inl h => simp [h.left]; omega
-            case inr h => simp [h.left]; omega
-        case neg h_k'_more =>
-            simp at h_step
-            left
-            simp [h_step]
-            omega
-    case neg h_k_j =>
-        simp at h_k_j
-        split_ifs at h_step
-        case pos h_k'_j =>
-            simp at h_step
-            cases h_step
-            case inl h_step =>
-                simp [h_step.left]
-                omega
-            case inr h_step =>
-                simp [h_step.left]
-                omega
-        case neg h_k'_j =>
-            simp at h_k'_j h_step ⊢
-            simp [h_step.left]
-            omega
-
-lemma regex_for_path_contains_kk (A : εNFA α ℕ) (i j k k' : ℕ) (h_k' : k' ≤ k) :
-    (to_trim A i j k).contains (to_trim A k k k') := by
-    simp [εNFA.contains]
-    intro q σ
-    rw [@subset_def]
-    intro t h_step
-    simp [to_trim] at h_step ⊢
-    split_ifs
-    case pos h_k_j =>
-        have h_k'_j: k' < j := by omega
-        simp
-        split_ifs at h_step
-        case pos h_k'_less =>
-            left
-            simp_all
-            cases h_step
-            case inl h => simp [h.left]; omega
-            case inr h => simp [h.left]; omega
-        case neg h_k'_more =>
-            simp at h_step
-            left
-            simp [h_step]
-            omega
-    case neg h_k_j =>
-        simp at h_k_j
-        split_ifs at h_step
-        case pos h_k'_j =>
-            simp at h_step
-            cases h_step
-            case inl h_step =>
-                simp [h_step.left]
-                omega
-            case inr h_step =>
-                simp [h_step.left]
-                omega
-        case neg h_k'_j =>
-            simp at h_k'_j h_step ⊢
-            simp [h_step.left]
-            omega
-
-lemma regex_for_path_kk_star_is_path_in_kk (A : εNFA α ℕ) (k : ℕ) (L': List (List (Option α))) :
-    (∀ (x' : List (Option α)), (x' ∈ L' → Nonempty (A.Path k k x'))) → Nonempty (A.Path k k L'.flatten) := by
-    intro h_y
-
-    induction L'
-    case nil =>
-        simp only [List.flatten_nil, εNFA.isPath_nil]
-    case cons head tail h_induction =>
-        have h_tail : (∀ y' ∈ tail, Nonempty (A.Path k k y')) := by
-            simp at h_y
-            exact h_y.right
-        apply h_induction at h_tail
-
-        simp only [List.flatten_cons]
-        apply A.isPath_append.mpr
-        use k
-        exact ⟨ by simp [h_y], h_tail ⟩
-
-lemma regex_for_path_contains_kj (A : εNFA α ℕ) (i j k k' : ℕ) (h_k' : k' ≤ k) :
-    (to_trim A i j k).contains (to_trim A k j k') := by
-    simp [εNFA.contains]
-    intro q σ
-    rw [@subset_def]
-    intro t h_step
-    simp [to_trim] at h_step ⊢
-    split_ifs
-    case pos h_k_j =>
-        have h_k'_j: k' < j := by omega
-        simp [h_k'_j] at h_step ⊢
-        cases h_step
-        case inl h_t_k' =>
-            left
-            simp [h_t_k']
-            omega
-        case inr h_t_j =>
-            right
-            exact h_t_j
-    case neg h_k_j =>
-        simp at h_k_j
-        split_ifs at h_step
-        case pos h_k'_j =>
-            simp at h_step
-            cases h_step
-            case inl h_step =>
-                simp [h_step.left]
-                omega
-            case inr h_step =>
-                simp [h_step.left]
-                omega
-        case neg h_k'_j =>
-            simp at h_k'_j h_step ⊢
-            simp [h_step.left]
-            omega
-
 lemma path_start_mem_supp
     (A : εNFA α ℕ) (s u : ℕ) (x : List (Option α))
     (p : A.Path s u x) :
-    s ∈ p.supp := by
+    x = [] ∨ s ∈ p.supp := by
         cases p with
-        | nil s =>
-            simp [εNFA.Path.supp]
+        | nil => left; rfl
         | cons t s u c tail h_step h_rest =>
+            right
             simp [εNFA.Path.supp]
 
 lemma not_none_is_some (c : Option α):
@@ -1034,76 +123,6 @@ lemma not_none_is_some (c : Option α):
     case none => contradiction
     case some σ => use σ
 
-lemma path_trim_of_not_mem_supp
-    (A : εNFA α ℕ) (i j k : ℕ)
-    (s u : ℕ) (x' : List (Option α))
-    (hk : k ≠ 0)
-    (p : (to_trim A i j k).Path s u x')
-    (h_not : k ∉ p.supp) :
-    Nonempty ((to_trim A i j (k - 1)).Path s u x') := by
-  revert h_not
-  induction p with
-  | nil s =>
-      intro h_not
-      exact (to_trim A i j (k - 1)).isPath_nil.mpr rfl
-
-  | cons t s u c tail h_step h_rest ih =>
-      intro h_not
-
-      have h_not_rest : k ∉ h_rest.supp := by
-            intro hk_rest
-            apply h_not
-            simp [εNFA.Path.supp, hk_rest]
-
-      have h_rest_small :
-          Nonempty ((to_trim A i j (k - 1)).Path t u tail) := by
-            exact ih h_not_rest
-
-      have h_t_not_k : t ≠ k := by
-            intro htk
-            subst t
-            exact h_not_rest (path_start_mem_supp (to_trim A i j k) k u tail h_rest)
-
-      have h_step_small :
-          t ∈ (to_trim A i j (k - 1)).step s c := by
-        simp [to_trim] at h_step
-        simp [to_trim]
-
-        by_cases h_old : (j > k)
-        · simp [h_old] at h_step
-          have hk_pos : 0 < k := by omega
-          have h_new : k - 1 < j := by
-            omega
-          simp [h_new]
-
-          rcases h_step with hcase1 | hcase2
-          · rcases hcase1 with ⟨hAstep, hbound⟩
-            left
-            refine ⟨hAstep, ?_⟩
-            omega
-          · rcases hcase2 with ⟨hAstep, htj⟩
-            right
-            refine ⟨hAstep, ?_⟩
-            exact htj
-
-        · simp [h_old] at h_step
-          by_cases h_new : (j > k - 1)
-          · simp [h_new]
-            rcases h_step with ⟨hAstep, hbound⟩
-            left
-            refine ⟨hAstep, ?_⟩
-            omega
-
-          · simp [h_new]
-            rcases h_step with ⟨hAstep, hbound⟩
-            refine ⟨hAstep, ?_⟩
-            omega
-
-      rw [← List.singleton_append]
-      apply (to_trim A i j (k - 1)).isPath_append.mpr
-      refine ⟨t, ?_, h_rest_small⟩
-      exact (to_trim A i j (k - 1)).isPath_singleton.mpr h_step_small
-
 lemma list_map_of_reduce_option (L' : List (List (Option α))) :
     L'.flatten.reduceOption = (List.map (fun x' ↦ x'.reduceOption) L').flatten := by
     induction L'
@@ -1111,6 +130,122 @@ lemma list_map_of_reduce_option (L' : List (List (Option α))) :
     case cons head tail h_induction =>
         simp [List.reduceOption_append]
         exact h_induction
+
+lemma supp_of_nil (A : εNFA α ℕ) (s t : ℕ) (path: A.Path s t []) : path.supp = ∅ := by
+    cases path
+    simp
+
+lemma supp_of_singleton (A : εNFA α ℕ) (s t : ℕ) (c: (Option α)) (path: A.Path s t [c]) : path.supp = {s} := by
+    cases path
+    next cons t' h_step path' =>
+    have : path'.supp = ∅ := supp_of_nil A t' t path'
+    simp [this]
+
+lemma path_split_at_state (A : εNFA α ℕ) (qs qf t : ℕ) (x': List (Option α)) (path_qs_qf: A.Path qs qf x') :
+    t ∈ path_qs_qf.supp → qs = t ∨
+    ∃ (y' : List (Option α)), ∃ (path_qs_t: A.Path qs t y'),
+     (Path.isPrefixOf A path_qs_t path_qs_qf) ∧
+     t ∉ path_qs_t.supp := by
+
+    intro h_t_in_path_qs_qf
+    induction path_qs_qf
+    case nil s =>
+        simp at h_t_in_path_qs_qf
+    case cons s qs qf c tail h_step path_s_qf h_induction =>
+        by_cases t = qs
+        case pos h => left; exact symm h
+        case neg h_qs_neq_t =>
+            right
+            have := A.isPath_singleton.mpr h_step
+            obtain ⟨ path_qs_s ⟩ := this
+            by_cases t = s
+            case pos h =>
+                clear h_induction
+                symm at h
+                subst h
+                use [c]
+                use path_qs_s
+                have : path_qs_s.supp = {qs} := supp_of_singleton A qs s c path_qs_s
+                simp [this, h_qs_neq_t]
+                unfold Path.isPrefixOf
+                split
+                case h_1 => contradiction
+                case h_2 => contradiction
+                case h_3 qs qf s t₁ s₁ x t₂ s₂ y t₁' s₁' path_y path_x u₁ c₁ y_tail u₂ c₂ x_tail h_eq₁ path_x_tail h_eq₂ path_y_tail _ _ h_path_y_tail h_path_x_tail =>
+                    simp at h_eq₁ h_eq₂
+                    obtain ⟨ h₁, h₂ ⟩ := h_eq₁
+                    subst h₁ h₂
+                    obtain ⟨ h₁, h₂ ⟩ := h_eq₂
+                    subst h₁ h₂
+                    simp_all
+                    obtain ⟨ h, h_path_x_tail ⟩ := h_path_x_tail
+                    subst h
+
+                    have := A.isPath_nil.mp (by use path_y_tail)
+                    subst this
+                    simp_all
+                    cases path_y_tail
+                    case nil =>
+                        unfold Path.isPrefixOf
+                        simp
+            case neg h_s_neq_t =>
+                simp[h_qs_neq_t] at h_t_in_path_qs_qf
+                replace h_induction := h_induction h_t_in_path_qs_qf
+                cases h_induction
+                case inl h => simp [symm h] at h_s_neq_t -- contradiction
+                case inr h_induction =>
+                    obtain ⟨ tail', path_s_t, h_tail'_prefix, h_supp ⟩ := h_induction
+                    let path_qs_t := Path.cons s qs t c tail' h_step path_s_t
+
+                    use [c] ++ tail', path_qs_t
+                    constructor
+                    case left =>
+                        unfold Path.isPrefixOf
+                        simp
+                        exact h_tail'_prefix
+                    case right =>
+                        subst path_qs_t
+                        simp [h_qs_neq_t, h_supp]
+
+lemma path_multiple_split_at_state (A : εNFA α ℕ) (i j k : ℕ) (x': List (Option α)) (path_ij: A.Path i j x'):
+    (k ∈ path_ij.supp) →
+    ∃ (word_ik word_kk word_kj : List (Option α))
+      (path_ik : A.Path i k word_ik) (path_kk : A.Path k k word_kk) (path_kj : A.Path k j word_kj),
+        Path.isEqv A path_ij (Path.append A (Path.append A path_ik path_kk) path_kj) ∧
+        (k ∉ path_ik.supp) ∧ (k ∉ (Path.states A path_kj).tail) := by
+    intro h_k_supp
+    induction path_ij
+    case nil => simp at h_k_supp
+    case cons t i j c tail h_step path_tj h_induction =>
+        simp at h_k_supp
+        cases h_k_supp
+        case inl h_ik =>
+            sorry
+        case inr h_k_supp =>
+            replace h_induction := h_induction h_k_supp
+            obtain ⟨ word_tk, word_kk, word_kj, path_tk, path_kk, path_kj,
+                     h_equiv, h_k_notin_path_tk, h_notin_path_kj_tail⟩ := h_induction
+            by_cases h_ik: k = i
+            case pos =>
+                subst h_ik
+                use [], [c] ++ word_tk ++ word_kk, word_kj
+                have h_path_ik : Nonempty (A.Path k k []) := A.isPath_nil.mpr rfl
+                obtain ⟨ path_ik ⟩ := h_path_ik
+                use path_ik, Path.cons t k k c (word_tk ++ word_kk) h_step (Path.append A path_tk path_kk), path_kj
+                simp_all
+                constructor
+                case left =>
+                    -- TODO
+                    sorry
+                case right =>
+                    cases path_ik
+                    case nil => simp
+            case neg =>
+                use [c] ++ word_tk, word_kk, word_kj
+                use Path.cons t i k c word_tk h_step path_tk, path_kk, path_kj
+                simp_all
+                sorry
+
 
 lemma regex_is_path_mp (A : εNFA α ℕ) (i j k : ℕ) (r: RegularExpression α) (hr: r = regex_for_path_from_i_to_j_through_k A i j k)
     (h_zero_step: ∀ (σ : Option α), A.step 0 σ = ∅) (h_step_zero: ∀ (q : ℕ) (σ : Option α), 0 ∉ A.step q σ):
@@ -1249,75 +384,6 @@ lemma regex_is_path_mp (A : εNFA α ℕ) (i j k : ℕ) (r: RegularExpression α
     --         refine ⟨ k, h_path_ik , ?_ ⟩
     --         apply (to_trim A i j k).isPath_append.mpr
     --         use k
-
-
-lemma path_prefix_of_state (A : εNFA α ℕ) (qs qf t : ℕ) (x': List (Option α)) (path_qs_qf: A.Path qs qf x') :
-    t ∈ path_qs_qf.supp → qs = t ∨
-        ∃ (y' : List (Option α)), y'.isPrefixOf x' ∧
-        ∃ (path_qs_t: A.Path qs t y'),
-        t ∉ path_qs_t.supp := by
-    intro h_t_in_path_qs_qf
-    induction path_qs_qf
-    case nil s =>
-        simp at h_t_in_path_qs_qf
-        subst h_t_in_path_qs_qf
-        simp
-    case cons s qs qf c tail h_step path_s_qf h_induction =>
-        by_cases t = qs
-        case pos h => left; exact symm h
-        case neg h_qs_neq_t =>
-            right
-            have := A.isPath_singleton.mpr h_step
-            obtain ⟨ path_qs_s ⟩ := this
-            by_cases t = s
-            case pos h =>
-                subst h
-                use [c]
-                simp
-                use path_qs_s
-                have : path_qs_s.supp = {qs} := by
-                    sorry -- TODO
-
-                simp [this, h_qs_neq_t]
-            case neg h_s_neq_t =>
-                simp[h_qs_neq_t] at h_t_in_path_qs_qf
-                replace h_induction := h_induction h_t_in_path_qs_qf
-                cases h_induction
-                case inl h => simp [symm h] at h_s_neq_t -- contradiction
-                case inr h_induction =>
-                    obtain ⟨ tail', h_tail'_prefix, path_s_t, h_supp ⟩ := h_induction
-                    use [c] ++ tail'
-                    simp [h_tail'_prefix]
-                    obtain ⟨ path_qs_t ⟩ := A.isPath_append.mpr ⟨ s, ⟨ path_qs_s ⟩ , ⟨ path_s_t ⟩ ⟩
-                    have : path_qs_s.supp = {qs} := by
-                        sorry -- TODO
-
-                    use path_qs_t
-                    sorry -- TODO union of supps
-
-open εNFA
-
-lemma split_path_by_state (A : εNFA α ℕ) (i j k : ℕ) (x': List (Option α)) (path_ij: A.Path i j x'):
-    (k ∈ path_ij.supp) → ∃ (steps_ik steps_kk steps_kj : List (ℕ × Option α × Prop)),
-        steps_ik ++ steps_kk ++ steps_kj = path_ij.steps ∧
-        (k ∉ (Path.steps.states steps_ik).tail) ∧ (k ∉ (Path.steps.states steps_kj).tail) := by
-    intro h_k_supp
-    induction path_ij
-    case nil s =>
-        use [(s, none, True)], [], []
-        simp [Path.steps.states]
-    case cons t s u c tail h_step path h_induction =>
-        by_cases k = s
-        case pos h_sk =>
-            subst h_sk
-            use [(k, none, True)]
-            by_cases k ∈ path.supp
-            case pos h_k_in_path =>
-                obtain ⟨ steps_ik, steps_kk, steps_kj, h_path, h ⟩ := h_induction h_k_in_path
-                use steps_ik ++ steps_kk, steps_kj
-                simp
-            case neg => sorry
-        case neg => sorry
 
 theorem regex_is_path (A : εNFA α ℕ) (i j k : ℕ) (r: RegularExpression α) (hr: r = regex_for_path_from_i_to_j_through_k A i j k)
     (h_zero_step: ∀ (σ : Option α), A.step 0 σ = ∅) (h_step_zero: ∀ (q : ℕ) (σ : Option α), 0 ∉ A.step q σ):
